update against new API + add to CoqProject. No lemma reproven yet.

examples/ping/interfaces.v
@@ -12,6 +12,7 @@ Local Obligation Tactic := simpl.
 
 Generalizable All Variables. 
 Local Open Scope monae_scope.
+Import FreerFuns.
 
 Create HintDb ping_db.
 
@@ -45,18 +46,22 @@ Inductive M := ping | pong.
 (* Client is described as :
  * C = send (ping); wait (pong).
  *)
-Inductive client_api : interface :=
+Inductive client_api : effect :=
 | SEND : M -> client_api unit
 | WAIT : client_api M.
 
-Definition send `{Provide ix client_api} {im : impureMonad ix} : im unit := trigger (im:=im) (inj_p $ SEND ping).
-Definition wait `{Provide ix client_api} {im : impureMonad ix} : im M := trigger (im:=im) (inj_p $ WAIT).
+Definition send `{Provide ix client_api} {im : freerMonad ix} : im unit :=
+  trigger (im:=im) (inj_p $ SEND ping).
+Definition wait `{Provide ix client_api} {im : freerMonad ix} : im M :=
+  trigger (im:=im) (inj_p $ WAIT).
 
-Definition C `{Provide ix client_api} {im : impureMonad ix} : im M := send >> wait.
+Definition C `{Provide ix client_api} {im : freerMonad ix} : im M :=
+  send >> wait.
 
 (* ======================================================================== *)
 
-Fixpoint loop `{Provide ix i} {im : impureMonad ix} (fuel : nat) `(prog : im X) : im unit := match fuel with 
+Fixpoint loop `{Provide ix i} {im : freerMonad ix} (fuel : nat) `(prog : im X)
+    : im unit := match fuel with
 | 0%nat => prog >> skip
 | S ful => prog >> loop ful prog
 end.
@@ -64,15 +69,19 @@ end.
 (* Server is described as :
  * S = μX. recv(ping); reply(pong); X.
  *)
-Inductive server_api : interface :=
+Inductive server_api : effect :=
 | RPLY : M -> server_api unit
 | RECV : server_api M.
 
-Definition reply `{Provide ix server_api} {im : impureMonad ix} : im unit := trigger (im:=im) (inj_p $ RPLY pong).
-Definition recv `{Provide ix server_api} {im : impureMonad ix} : im M := trigger (im:=im) (inj_p $ RECV).
+Definition reply `{Provide ix server_api} {im : freerMonad ix} : im unit :=
+  trigger (im:=im) (inj_p $ RPLY pong).
+Definition recv `{Provide ix server_api} {im : freerMonad ix} : im M :=
+  trigger (im:=im) (inj_p $ RECV).
 
-Definition S_p `{Provide ix server_api} {im : impureMonad ix} : im unit := recv >> reply.
-Definition S_ `{Provide ix server_api} {im : impureMonad ix} (fuel : nat) : im unit := loop fuel S_p.
+Definition S_p `{Provide ix server_api} {im : freerMonad ix} : im unit :=
+  recv >> reply.
+Definition S_ `{Provide ix server_api} {im : freerMonad ix} (fuel : nat)
+    : im unit := loop fuel S_p.
 
  
 (* ======================================================================== *)
@@ -87,7 +96,8 @@ Record N := mk_chan {
 }.
 
 
-Definition send_over_network (m : M) (n : N) := {| tx := m :: (tx n) ; rx := rx n|}.
+Definition send_over_network (m : M) (n : N) :=
+  {| tx := m :: tx n; rx := rx n |}.
 Definition consume_received (n : N) := match rx n with
 | [::] => {| tx := tx n ; rx := [::] |}
 | _ :: ns => {| tx := tx n ; rx := ns |}
@@ -110,18 +120,19 @@ Import NetworkChannelMod.
 Module ccm.
   Section ccs.
     (* make_contract
-     : forall (i : interface) (Ω : UU0),
+     : forall (i : effect) (Ω : UU0),
 (Ω -> forall α : UU0, i α -> α -> Ω) ->
 (Ω -> forall α : UU0, i α -> Prop) ->
 (Ω -> forall α : UU0, i α -> α -> Prop) -> contract i Ω *)
 
-      Definition c_step (network : N) : forall X, client_api X -> X -> N := fun X ec x =>
-      match ec with
-      | SEND m => send_over_network m network
-        (* add packet tx *)
-      | WAIT => consume_received network 
-        (* remove packet rx (if present) *)
-      end.
+      Definition c_step (network : N) : forall X, client_api X -> X -> N :=
+        fun X ec x =>
+          match ec with
+          | SEND m => send_over_network m network
+            (* add packet tx *)
+          | WAIT => consume_received network
+            (* remove packet rx (if present) *)
+          end.
 
       Inductive c_o_caller (st : N) : forall X, client_api X -> Prop :=
       | O_WAIT (equ : forall ns, ping :: ns = st.(tx)) : c_o_caller st WAIT
@@ -132,38 +143,51 @@ Module ccm.
     Check head.
     (* Search (seq _ -> ) *)
       Inductive c_o_callee (st : N) : forall X, client_api X -> X -> Prop :=
-      | SEND_O (u : unit) (m : M) (equ_m : m = ping) (equ : forall ns, m :: ns = st.(tx)) : c_o_callee st (SEND m) u
+      | SEND_O (u : unit) (m : M) (equ_m : m = ping)
+          (equ : forall ns, m :: ns = st.(tx)) : c_o_callee st (SEND m) u
       | WAIT_O : c_o_callee st WAIT pong
-      (* | WAIT_O (m : M) (msg_output : m = pong) (equ : first_not_from_me from st) : c_o_callee from to st WAIT m *)
-      (* | SEND_O (u : unit) (equ : Some ping = (peek_first st).(message)) : c_o_callee from to st (SEND ping) u *)
-      . 
+      (* | WAIT_O (m : M) (msg_output : m = pong)
+           (equ : first_not_from_me from st) : c_o_callee from to st WAIT m *)
+      (* | SEND_O (u : unit) (equ : Some ping = (peek_first st).(message))
+           : c_o_callee from to st (SEND ping) u *)
+      .
       Hint Constructors c_o_callee : ping_db.
 
-      Definition c_contract := make_contract c_step no_caller_obligation (c_o_callee).
+      Definition c_contract :=
+        make_contract c_step no_caller_obligation c_o_callee.
 
       (* Safety *)
-      Lemma c_respect `{Provide ix client_api} {im : impureMonad ix} (network : N)
-        : pre (to_hoare (im:=ImpureModule_acto__canonical__Impure_MonadImpure ix) (c_contract) (C)) network.
+      Lemma c_respect `{Provide ix client_api} {im : freerMonad ix}
+          (network : N)
+        : pre (to_hoare (im:=im) c_contract C) network.
+      (*
       Proof.
-         prove impure with ping_db.
+        prove impure with ping_db.
       Qed.
+      *)
+      Admitted.
 
       (* Liveness *)
-      Lemma c_run `{Provide ix client_api} {im : impureMonad ix} (initial_network final_network : N) (m : M)
-        (run : post (to_hoare (im:=ImpureModule_acto__canonical__Impure_MonadImpure ix) (c_contract) (C)) initial_network m final_network)
+      Lemma c_run `{Provide ix client_api} {im : freerMonad ix}
+          (initial_network final_network : N) (m : M)
+        (run : post (to_hoare (im:=im) c_contract C)
+          initial_network m final_network)
         : m = pong.
+      (*
       Proof.
-        (* Tactic `unroll_post` needs to be reworked to do this automatically. *)
-  by run_simpl run;
-  cleanvert H1;
-  simplify_gens;
-  destruct run as [wait_callee wait_state];
-  simplify_gens;
-  inversion wait_callee; subst;
-  cleanvert wait_state; cleanvert H1; cleanvert H2; cleanvert H3;
-  simplify_gens;
-  cleanvert H1.
+        (* Tactic `unroll_post` needs to be reworked automatically. *)
+        by run_simpl run;
+          cleanvert H1;
+          simplify_gens;
+          destruct run as [wait_callee wait_state];
+          simplify_gens;
+          inversion wait_callee; subst;
+          cleanvert wait_state; cleanvert H1; cleanvert H2; cleanvert H3;
+          simplify_gens;
+          cleanvert H1.
       Qed.
+      *)
+      Admitted.
   End ccs.
 End ccm.
 
@@ -174,11 +198,12 @@ Module scm.
   Section scs.
 
 
-      Definition s_step (network : N) : forall X, server_api X -> X -> N := fun X ec x =>
-      match ec with
-      | RPLY m => send_over_network m network
-      | RECV   => consume_received network
-      end.
+      Definition s_step (network : N) : forall X, server_api X -> X -> N :=
+        fun X ec x =>
+          match ec with
+          | RPLY m => send_over_network m network
+          | RECV => consume_received network
+          end.
 
       Inductive s_o_caller (st : N) : forall X, server_api X -> Prop :=
       | O_RECV (*blocking : rx st <> [::]*) : s_o_caller st RECV
@@ -195,17 +220,24 @@ Module scm.
       Definition s_contract := make_contract s_step s_o_caller s_o_callee.
 
 
-      Lemma s_respect `{Provide ix server_api} {im : impureMonad ix} (network : N) fuel
-        : pre (to_hoare (im:=ImpureModule_acto__canonical__Impure_MonadImpure ix) s_contract (S_ fuel)) network.
+      Lemma s_respect `{Provide ix server_api} {im : freerMonad ix}
+          (network : N) fuel
+        : pre (to_hoare (im:=im) s_contract (S_ fuel)) network.
+      (*
       Proof.
-        move : network; 
+        move : network;
           elim : fuel => [|ful EH] network;
           prove impure with ping_db; constructor.
       Qed.
+      *)
+      Admitted.
 
-      Lemma s_p_run_grows `{Provide ix server_api} {im : impureMonad ix} (initial_network final_network : N) (u : unit)
-        (run : post (to_hoare (im:=ImpureModule_acto__canonical__Impure_MonadImpure ix) s_contract S_p) initial_network u final_network)
+      Lemma s_p_run_grows `{Provide ix server_api} {im : freerMonad ix}
+          (initial_network final_network : N) (u : unit)
+        (run : post (to_hoare (im:=im) s_contract S_p)
+          initial_network u final_network)
         : tx final_network = pong :: tx initial_network.
+      (*
       Proof.
         (* Should be :
         by unroll_post run;
@@ -218,22 +250,34 @@ Module scm.
           case : run => [reply_callee reply_state];
           simplify_gens;
           inversion reply_callee; subst;
-          cleanvert reply_state; cleanvert H1; cleanvert H2; cleanvert H3; simplify_gens; cleanvert H1;
+          cleanvert reply_state; cleanvert H1; cleanvert H2; cleanvert H3;
+          simplify_gens; cleanvert H1;
           rewrite /= consuming_has_no_effect_on_tx.
       Qed.
+      *)
+      Admitted.
 
-      Lemma s_run `{Provide ix server_api} {im : impureMonad ix} (initial_network final_network : N) (u : unit) fuel
-        (run : post (to_hoare (im:=ImpureModule_acto__canonical__Impure_MonadImpure ix) s_contract (S_ fuel)) initial_network u final_network)
+      Lemma s_run `{Provide ix server_api} {im : freerMonad ix}
+          (initial_network final_network : N) (u : unit) fuel
+        (run : post (to_hoare (im:=im) s_contract (S_ fuel))
+          initial_network u final_network)
         : tx final_network = nseq (S fuel) pong ++ tx initial_network.
+      (*
       Proof.
         move : initial_network final_network u run.
         elim : fuel => [|fuel IH] initial_network final_network u.
         - (* Should be : by unroll_post; rewrite (s_p_run_grows run_p). *)
-          by move => /(to_hoare_post_bind_assoc s_contract (S_p (im:=ImpureModule_acto__canonical__Impure_MonadImpure ix)) (fun _ : unit => skip (M:=ImpureModule_acto__canonical__Impure_MonadImpure ix)))
+          by move => /(to_hoare_post_bind_assoc s_contract
+            (S_p (im:=ImpureModule_acto__canonical__Impure_MonadImpure ix))
+            (fun _ : unit =>
+              skip (M:=ImpureModule_acto__canonical__Impure_MonadImpure ix)))
             [x [middle_network [run_p run_skip]]];
             run_simpl run_skip;
             rewrite (s_p_run_grows run_p).
-        move=> /(to_hoare_post_bind_assoc s_contract (S_p (im:=ImpureModule_acto__canonical__Impure_MonadImpure ix)) (fun _ : unit => S_ (im:=ImpureModule_acto__canonical__Impure_MonadImpure ix) fuel))
+        move=> /(to_hoare_post_bind_assoc s_contract
+          (S_p (im:=ImpureModule_acto__canonical__Impure_MonadImpure ix))
+          (fun _ : unit =>
+            S_ (im:=ImpureModule_acto__canonical__Impure_MonadImpure ix) fuel))
             [x [middle_network [run_p run_loop]]];
             rewrite /= (IH _ _ _ run_loop) (s_p_run_grows run_p) //;
             clear IH run_loop run_p.
@@ -245,16 +289,24 @@ Module scm.
 
         exact: nseq_pong_cons.
       Qed.
+      *)
+      Admitted.
 
-      Lemma s_run_size `{Provide ix server_api} {im : impureMonad ix} (initial_network final_network : N) (u : unit) fuel
-        (run : post (to_hoare (im:=ImpureModule_acto__canonical__Impure_MonadImpure ix) s_contract (S_ fuel)) initial_network u final_network)
+      Lemma s_run_size `{Provide ix server_api} {im : freerMonad ix}
+          (initial_network final_network : N) (u : unit) fuel
+        (run : post (to_hoare (im:=im) s_contract (S_ fuel))
+          initial_network u final_network)
         : size (tx final_network) = size (tx initial_network) + fuel + 1.
+      (*
       Proof.
         have -> : tx final_network = nseq (S fuel) pong ++ tx initial_network
-          := s_run (im:=im) (initial_network:=initial_network) (final_network:=final_network) (u:=u) (fuel:=fuel) run. 
+          := s_run (im:=im) (initial_network:=initial_network)
+            (final_network:=final_network) (u:=u) (fuel:=fuel) run.
         rewrite size_cat size_nseq;
           lia.
       Qed.
+      *)
+      Admitted.
 
   End scs.
 End scm.
